theories/iris/logrel/instr/typing/case.v
@@ -1,4 +1,5 @@
 Require Import RichWasm.iris.logrel.instr.typing.common.
+Require Import RichWasm.util.
 
 Set Bullet Behavior "Strict Subproofs".
 Set Default Goal Selector "!".
@@ -385,11 +386,9 @@ Proof.
 
     clear_nils.
 
-    inv_cg_bind Hcg ?units ?wt ?wt ?wl ?wl ?es es_case1 Hcases Hret.
-    inv_cg_ret Hret; subst.
+    inv_cg_bind Hcg [] ?wt ?wt ?wl ?wl ?es es_case2 Hcase_es1 Hcase_es2.
 
     (* Case es1 *)
-    inv_cg_bind Hcases [] ?wt ?wt ?wl ?wl ?es es_case2 Hcase_es1 Hcase_es2.
 
     inv_cg_bind Hcase_es1 ?pair ?wt ?wt ?wl ?wl ?es ?es Hcase_es1 Hcase_es1_block.
     destruct pair, u.
@@ -427,9 +426,8 @@ Proof.
     clear_nils.
 
     (* Case es2 *)
+
     inv_cg_bind Hcase_es2 ?units ?wt ?wt ?wl ?wl ?es ?es Hcase_es2 Hmret.
-    inv_cg_ret Hmret; subst.
-    inv_cg_bind Hcase_es2 [] ?wt ?wt ?wl ?wl ?es ?es Hcase_es2 Hmret.
     inv_cg_ret Hmret; subst.
 
     inv_cg_bind Hcase_es2 ?pair ?wt ?wt ?wl ?wl ?es ?es Hcase_es2 Hcase_es2_block.
@@ -816,11 +814,10 @@ Proof.
 
     clear_nils.
 
-    inv_cg_bind Hcg ?units ?wt ?wt ?wl ?wl ?es es_case1 Hcases Hret.
-    inv_cg_ret Hret; subst.
+    inv_cg_bind Hcg [] ?wt ?wt ?wl ?wl ?es es_case2 Hcase_es1 Hcases.
+    inv_cg_bind Hcases [] ?wt ?wt ?wl ?wl ?es ?es Hcase_es2 Hcase_es3.
 
     (* Case es1 *)
-    inv_cg_bind Hcases [] ?wt ?wt ?wl ?wl ?es es_case2 Hcase_es1 Hcase_es2.
 
     inv_cg_bind Hcase_es1 ?pair ?wt ?wt ?wl ?wl ?es ?es Hcase_es1 Hcase_es1_block.
     destruct pair, u.
@@ -858,9 +855,6 @@ Proof.
     clear_nils.
 
     (* Case es2 *)
-    inv_cg_bind Hcase_es2 ?units ?wt ?wt ?wl ?wl ?es ?es Hcase_es2 Hmret.
-    inv_cg_ret Hmret; subst.
-    inv_cg_bind Hcase_es2 [] ?wt ?wt ?wl ?wl ?es ?es Hcase_es2 Hcase_es3.
 
     inv_cg_bind Hcase_es2 ?pair ?wt ?wt ?wl ?wl ?es ?es Hcase_es2 Hcase_es2_block.
     destruct pair, u.
@@ -898,8 +892,6 @@ Proof.
 
     (* Case es3 *)
     inv_cg_bind Hcase_es3 ?units ?wt ?wt ?wl ?wl ?es ?es Hcase_es3 Hmret.
-    inv_cg_ret Hmret; subst.
-    inv_cg_bind Hcase_es3 [] ?wt ?wt ?wl ?wl ?es ?es Hcase_es3 Hmret.
     inv_cg_ret Hmret; subst.
 
     inv_cg_bind Hcase_es3 ?pair ?wt ?wt ?wl ?wl ?es ?es Hcase_es3 Hcase_es3_block.
@@ -1307,6 +1299,21 @@ Proof.
         rewrite length_app. lia.
   Admitted.
 
+
+  Lemma compile_cases_app fe ess1 ess2 :
+    (fix compile_cases fe ess := match ess with
+     | [] => [] | es :: ess' => mapM_ (compile_instr mr fe) es :: compile_cases fe ess'
+     end) fe (ess1 ++ ess2) =
+    (fix compile_cases fe ess := match ess with
+     | [] => [] | es :: ess' => mapM_ (compile_instr mr fe) es :: compile_cases fe ess'
+     end) fe ess1 ++
+    (fix compile_cases fe ess := match ess with
+     | [] => [] | es :: ess' => mapM_ (compile_instr mr fe) es :: compile_cases fe ess'
+     end) fe ess2.
+  Proof.
+    induction ess1; simpl; [done | by rewrite IHess1].
+  Qed.
+
   Lemma compat_case M F L L' wt wt' wtf wl wl' wlf es' ess τs τs' κ :
     let fe := fe_of_context F in
     let WT := wt ++ wt' ++ wtf in
@@ -1327,6 +1334,602 @@ Proof.
     has_instruction_type_ok F ψ L' ->
     run_codegen (compile_instr mr fe (ICase ψ L' ess)) wt wl = inr ((), wt', wl', es') ->
     ⊢ have_instr_type_sem rti sr mr M F L WT WL lmask es' ψ L'.
+  Proof.
+    intros fe WT WL lmask F' Ψ Hforall Hok Hcg.
+    subst Ψ.
+    cbn [compile_instr] in Hcg.
+    destruct κ as [ ρ rf | ]; last inversion Hcg.
+    destruct ρ  as [ | ρs_sum | | ]; try done.
+    destruct τs' as [ | τ_res τs' ]; first done.
+    destruct τs'; last done.
+
+    inv_cg_bind Hcg wl_ret ?wt ?wt ?wl ?wl ?es ?es Hres_type Hcg.
+    inv_cg_try_option Hres_type; subst.
+
+    destruct (Wasm_int.Int32.modulus <? length ρs_sum)%Z eqn:Hcmp; first inversion Hcg.
+    inv_cg_bind Hcg ?units ?wt ?wt ?wl ?wl ?es es_case1 Hret Hcg.
+    inv_cg_ret Hret; subst.
+    apply Z.ltb_ge in Hcmp.
+
+    inv_cg_bind Hcg ρs_atom ?wt ?wt ?wl ?wl ?es ?es Hιs Hcg.
+    inv_cg_try_option Hιs; subst.
+    inv_cg_bind Hcg val_localidxs wt_save ?wt wl_save ?wl es_save ?es Hsave Hcg.
+    repeat rewrite app_nil_r in Hsave.
+
+    (* Save tag *)
+    inv_cg_bind Hcg tag_localidx ?wt ?wt ?wl ?wl ?es ?es HsaveTag Hcg.
+    unfold save_stack1 in HsaveTag.
+    inv_cg_bind HsaveTag ?tl ?wt ?wt ?wl ?wl ?es ?es Halloc_tag HsaveTag.
+    apply wp_wlalloc in Halloc_tag as [Hlocal_tag_idx [-> [-> ->]]].
+    inv_cg_bind HsaveTag [] ?wt ?wt ?wl ?wl es_set_tag ?es HsetTag HretTagIdx.
+    inv_cg_emit HsetTag; subst.
+    inv_cg_ret HretTagIdx; subst.
+
+    clear_nils.
+    set (tag_idx := (fe_wlocal_offset fe + length (wl ++ wl_save))).
+    set (tag_localidx := Mk_localidx tag_idx).
+    replace (Mk_localidx (fe_wlocal_offset fe + length (wl ++ wl_save))) with tag_localidx in *; last done.
+
+    (* Put default result values on stack *)
+    inv_cg_bind Hcg [] ?wt ?wt ?wl ?wl es_create_defaults ?es Hcreate_defaults Hcg.
+    apply run_codegen_create_defaults in Hcreate_defaults as H.
+    destruct H as (_ & -> & -> & _).
+
+    subst WT WL.
+    clear_nils.
+    simplify_eq.
+
+    (* Iris Proof *)
+    iIntros (? ? ? ? ? ? ? ?) "%Hsem %Hhas_values #Hinst #Hlabels #Hreturn Hrvs Hvs Hframe Hrt Hfr Hrun".
+
+    (* Our values are in the value interpretation for our specific SumT *)
+    (* This means that the values represent the tag and the payload. *)
+    iDestruct (values_interp_one_eq with "Hvs") as "Hvs".
+    iDestruct (value_interp_eq with "Hvs") as "Hvs".
+    unfold value_interp0, value_se_interp0.
+    iDestruct "Hvs" as "(%κ & %Hkind_sum & Hskind_as_type & Hsum_interp)".
+    (*unfold type_skind in Hkind_sum.*)
+    iDestruct "Hsum_interp" as (tag os' os_tag τ_tag ιs ιs_tag ixs  HSAtoms Htag_type_lookup Htag_type_arep Heval_rep_tail Hinject_sum_arep Hos'_ixs) "Hvalue_interp_os_i".
+    simplify_eq.
+
+    apply lookup_lt_Some in Htag_type_lookup as Htag_size_bound.
+    assert (length τs = length ρs_sum) as Htyp_rep_len.
+    {
+      inversion Hok; subst.
+      unfold has_mono_rep_instr in H.
+      destruct H as [H _].
+      simpl in H.
+      rewrite Forall_singleton in H.
+      inversion H; subst.
+      inversion H1; subst.
+      apply has_kind_SumT_inv in H3 as (rf' & HF2).
+      by eapply Forall2_length.
+    }
+    assert (tag < Wasm_int.Int32.modulus)%Z as Htag_in_i32_bound.
+    { rewrite Htyp_rep_len in Htag_size_bound. eapply Z.lt_le_trans; last done. by apply Nat2Z.inj_lt. }
+
+    iDestruct (big_sepL2_length with "Hrvs") as "%Hlen".
+    destruct vs as [|v_tag vs_payload]; first inversion Hlen.
+    clear Hlen.
+    iDestruct (atoms_interp_cons with "Hrvs") as "[-> Hatoms_interp_payload]".
+
+    iPoseProof (frame_interp_wl_interp with "Hframe") as "%Hwl"; first done.
+    rewrite list_extra.cons_app in Hhas_values.
+    apply has_values_app_inv in Hhas_values as (e_tag & es_payload & -> & Hhv_tag & Hhvs_payload).
+
+    (* tag is an index into τs, so we must have: *)
+    (* τs = τs_pre ++ [τ_tag] ++ τs_post *)
+    (* ess = ess_pre ++ [es_tag] ++ ess_post *)
+    apply list_elem_of_split_length in Htag_type_lookup as H.
+    destruct H as (τs_pre & τs_post & Hτs_eq & Htag_len).
+
+    rewrite Hτs_eq in Hforall.
+    apply Forall2_app_inv_l in Hforall as
+      (ess_pre & ess_rest & Hforall_pre & Hforall_rest & ->).
+    apply Forall2_cons_inv_l in Hforall_rest as
+      (es_tag & ess_post & Hforall_tag & Hforall_post & ->).
+
+
+    (* save payload *)
+    rewrite (app_assoc (e_tag ++ _)).
+    iApply (cwp_seq with "[Hfr Hrun]").
+    {
+      rewrite <- (app_assoc e_tag).
+      instantiate (1 := λ fr' vs, (
+        ∃ val_idxs,
+        ⌜vs = [VAL_int32 (Wasm_int.Int32.repr tag)]⌝ ∗
+        ⌜frame_rel (λ i, i ∉ val_idxs) fr fr'⌝ ∗
+        ⌜Forall2 (fun i v => f_locs fr' !! localimm i = Some v) val_localidxs vs_payload⌝ ∗
+        ⌜val_idxs = seq (fe_wlocal_offset fe + length wl) (length wl_save)⌝ ∗
+        ⌜val_localidxs = map prelude.W.Mk_localidx val_idxs⌝
+        )%I).
+      iApply cwp_val_app; first done.
+      eapply cwp_save_stack_w in Hsave; eauto.
+      + destruct Hsave as (-> & -> & -> & Hsave).
+        iApply (Hsave with "[$] [$]").
+        iIntros (f' [Hfsame Hfchanged]).
+        unfold fvs_combine.
+        auto.
+      + admit. (* easy pure conseqeunce of value_interp and
+      rep_values_interp, should be proved above the first wp_seq
+      rule *)
+    }
+    iIntros (fr_saved w) "(%val_idxs & -> & %Hfrel_fr_saved & %Hsaved & %Hval_idxs_seq & %Hval_localidxs) Hfr Hrun".
+    iAssert
+    (frame_interp rti sr se L (wl ++ wl_save ++ [prelude.W.T_i32] ++ wl1 ++ wlf) fr_saved)
+      with "[Hframe]" as "Hframe_saved".
+    { admit. } (* TODO: Not really sure how to prove this. Definitely need helper lemma *)
+
+    (* edestruct (util.nths_error_exists val_localidxs case_i_val_idxs vs_payload case_i_sum_locals (Forall2_length _ _ _ Hsaved)) as [case_i_vs_payload Hnerr_payload_ci]; try done. *)
+
+    iDestruct (frame_interp_wl_interp with "Hframe_saved") as "%Hwl_saved"; first done.
+    pose proof (interp_wl_length _ _ _ Hwl_saved) as Hfr_saved_locs_len.
+
+    assert (tag_idx < length (f_locs fr_saved)) as Htag_in_fr_saved.
+    {
+      subst tag_idx.
+      simpl.
+      eapply Nat.lt_le_trans; last done.
+      - rewrite app_assoc.
+        subst fe.
+        instantiate (1 := F).
+        repeat rewrite length_app.
+        lias.
+    }
+
+    (* Store tag *)
+    rewrite (app_assoc (map _ _)).
+    iApply (cwp_seq with "[Hfr Hrun]").
+    {
+      instantiate (1 := λ fr' vs, (
+        ⌜vs = []⌝ ∗
+        ⌜frame_rel (λ j, j ≠ tag_idx) fr_saved fr'⌝ ∗
+        ⌜f_locs fr' !! tag_idx = Some (VAL_int32 (Wasm_int.Int32.repr tag))⌝
+        )%I).
+      iApply (cwp_local_set with "[] [$] [$]"); first done.
+      iSplit; first done.
+      iSplit.
+      - iPureIntro.
+        split; last done.
+        intros j Hneq.
+        simpl.
+        rewrite list_lookup_insert_ne; [reflexivity | lia].
+      - iSimpl.
+        iPureIntro.
+        rewrite list_lookup_insert_eq; try done.
+    }
+    iIntros (fr_saved_and_tag w) "(-> & %Hfrel_fr_saved_and_tag & %Hsaved_and_tag) Hfr Hrun".
+    clear_nils.
+
+    (* relate starting frame fr and fr_saved_and_tag *)
+    pose proof (frame_rel_mask_trans_combine _ _ _ _ _ Hfrel_fr_saved Hfrel_fr_saved_and_tag) as Hfrel_fr_and_fr_saved_and_tag.
+    simpl in Hfrel_fr_and_fr_saved_and_tag.
+
+    assert (frame_rel lmask fr fr_saved_and_tag) as Hfrel_lmask_saved_and_tag.
+    {
+      eapply frame_rel_mask_mono; [| exact Hfrel_fr_and_fr_saved_and_tag].
+      intros i [Hi_lo Hi_hi].
+      split.
+      + rewrite Hval_idxs_seq.
+        intro Hin. apply elem_of_seq in Hin. lia.
+      + unfold tag_idx. rewrite length_app. lia.
+    }
+    pose proof Hfrel_fr_and_fr_saved_and_tag as [_ ->].
+    iDestruct (labels_interp_mono _ _ _ _ fr_saved_and_tag _ _ _ _ with "Hlabels") as "Hlabels'"; first done.
+    {
+      instantiate (1 := (wlmask (fe_of_context F') (wl ++ wl_save ++ [prelude.W.T_i32]))).
+      intros i [Hi_lo Hi_hi].
+      simpl.
+      split.
+      + exact Hi_lo.
+      + rewrite -fe_of_context_labels.
+        rewrite !length_app. simpl.
+        subst fe.
+        lia.
+    }
+
+    assert (Forall2 (λ (i : prelude.W.localidx) (v : value), f_locs fr_saved_and_tag !! localimm i = Some v)
+      val_localidxs vs_payload) as Hfr_saved_and_tag_payload.
+    {
+      eapply forall2_lookup_same.
+      3: done.
+      - intros j Hneq. instantiate (1 := tag_idx) in Hneq.
+        destruct Hfrel_fr_saved_and_tag as [-> _]; done.
+      - subst val_idxs val_localidxs tag_idx.
+        rewrite length_app Nat.add_assoc.
+        apply map_seq_forall_localidx_neq.
+    }
+
+    iAssert
+    (frame_interp rti sr se L (wl ++ wl_save ++ [prelude.W.T_i32] ++ wl1 ++ wlf) fr_saved_and_tag)
+      with "[Hframe_saved]" as "Hframe_saved_and_tag".
+    { admit. } (* TODO: Not really sure how to prove this. Definitely need helper lemma *)
+
+    (* Create defaults *)
+    iApply (cwp_seq with "[Hfr Hrun]").
+    {
+      eapply cwp_create_defaults in Hcreate_defaults as (_ & _ & _ & Hcreate_defaults).
+      iDestruct (Hcreate_defaults with "[$] [$] []") as "Hcreate_defaults".
+      {
+        by instantiate (1 := λ f vs, (⌜f = fr_saved_and_tag⌝ ∗ ⌜vs = (map default_of_value_type wl_ret)⌝)%I).
+      }
+      iApply "Hcreate_defaults".
+    }
+    iIntros (??) "[-> ->] Hfr Hrun".
+
+    rewrite compile_cases_app in Hcg.
+    rewrite map_app in Hcg.
+    rewrite map_cons in Hcg.
+    rewrite separate1 in Hcg.
+    apply run_codegen_case_blocks_blocks_app in Hcg as (wt_pre & wt_tag & wt_post & wl_pre & wl_tag & wl_post & es_pre & es_tag_cg & es_post & Hcg_pre & Hcg_tag & Hcg_post & -> & -> & ->).
+
+    (* (* Case blocks *) *)
+    (* cbv [map length seq zip Datatypes.uncurry] in Hcg. *)
+    (**)
+    (* clear_nils. *)
+    (**)
+    (* inv_cg_bind Hcg ?units ?wt ?wt ?wl ?wl ?es es_case_i Hcases Hret. *)
+    (* inv_cg_ret Hret; subst. *)
+    (**)
+    (* (* Case es_i *) *)
+    (* inv_cg_bind Hcases [] ?wt ?wt ?wl ?wl ?es es_rest Hcase_es_i Hrest. *)
+    (**)
+    (* inv_cg_bind Hcase_es_i ?pair ?wt ?wt ?wl ?wl ?es ?es Hcase_es_i Hcase_es_i_block. *)
+    (* destruct pair, u. *)
+    (* inv_cg_emit Hcase_es_i_block; subst. *)
+    (* apply run_codegen_capture in Hcase_es_i as [Hcase_es_i ->]. *)
+    (**)
+    (* inv_cg_bind Hcase_es_i [] ?wt ?wt ?wl ?wl ?es ?es Hget_tag Hcase_es_i. *)
+    (* inv_cg_emit Hget_tag; subst. *)
+    (**)
+    (* inv_cg_bind Hcase_es_i [] ?wt ?wt ?wl ?wl ?es ?es Htag0 Hcase_es_i. *)
+    (* inv_cg_emit Htag0; subst. *)
+    (**)
+    (* inv_cg_bind Hcase_es_i [] ?wt ?wt ?wl ?wl ?es ?es Hcompare_tag Hcase_es_i. *)
+    (* inv_cg_emit Hcompare_tag; subst. *)
+    (**)
+    (* inv_cg_bind Hcase_es_i [] ?wt ?wt ?wl ?wl ?es ?es Hbr_case Hcase_es_i. *)
+    (* inv_cg_emit Hbr_case; subst. *)
+    (**)
+    (* inv_cg_bind Hcase_es_i [] ?wt ?wt ?wl ?wl es_drop_i ?es Hdrop_consts_i Hcase_es_i. *)
+    (* apply run_codegen_drop_consts in Hdrop_consts_i as H. *)
+    (* destruct H as (_ & -> & -> & _). *)
+    (**)
+    (* inv_cg_bind Hcase_es_i ρ_casei ?wt ?wt ?wl ?wl ?es ?es Hlookup Hcase_es_i. *)
+    (* inv_cg_try_option Hlookup; subst. *)
+    (**)
+    (* inv_cg_bind Hcase_es_i case_i_sum_locals ?wt ?wt ?wl ?wl ?es ?es Hinject Hcase_es_i. *)
+    (* inv_cg_try_option Hinject; subst. *)
+    (**)
+    (* inv_cg_bind Hcase_es_i [] ?wt wt_case_i ?wl wl_case_i ?es es_case_i Hget_locals_i Hcase_es_i. *)
+    (* inv_cg_bind Hget_locals_i case_i_val_idxs ?wt wt_get_locals_i ?wl wl_get_locals_i ?es es_get_locals_i Hnths_error Hget_locals_i. *)
+    (* inv_cg_try_option Hnths_error; subst. *)
+    (**)
+    (* destruct (run_codegen_get_locals _ _ _ _ _ _ _ Hget_locals_i) as ([] & -> & ->). *)
+    (**)
+    (* (* clean up *) *)
+    (* subst WT WL. *)
+    (* clear_nils. *)
+    (* simplify_eq. *)
+    (**)
+    (**)
+    (* (* save payload *) *)
+    (* rewrite (app_assoc (e_tag ++ _)). *)
+    (* iApply (cwp_seq with "[Hfr Hrun]"). *)
+    (* { *)
+    (*   rewrite <- (app_assoc e_tag). *)
+    (*   instantiate (1 := λ fr' vs, ( *)
+    (*     ∃ val_idxs, *)
+    (*     ⌜vs = [VAL_int32 (Wasm_int.Int32.repr tag)]⌝ ∗ *)
+    (*     ⌜frame_rel (λ i, i ∉ val_idxs) fr fr'⌝ ∗ *)
+    (*     ⌜Forall2 (fun i v => f_locs fr' !! localimm i = Some v) val_localidxs vs_payload⌝ ∗ *)
+    (*     ⌜val_idxs = seq (fe_wlocal_offset fe + length wl) (length wl_save)⌝ ∗ *)
+    (*     ⌜val_localidxs = map prelude.W.Mk_localidx val_idxs⌝ *)
+    (*     )%I). *)
+    (*   iApply cwp_val_app; first done. *)
+    (*   eapply cwp_save_stack_w in Hsave; eauto. *)
+    (*   + destruct Hsave as (-> & -> & -> & Hsave). *)
+    (*     iApply (Hsave with "[$] [$]"). *)
+    (*     iIntros (f' [Hfsame Hfchanged]). *)
+    (*     unfold fvs_combine. *)
+    (*     auto. *)
+    (*   + admit. (* easy pure conseqeunce of value_interp and *)
+    (*   rep_values_interp, should be proved above the first wp_seq *)
+    (*   rule *) *)
+    (* } *)
+    (* iIntros (fr_saved w) "(%val_idxs & -> & %Hfrel_fr_saved & %Hsaved & %Hval_idxs_seq & %Hval_localidxs) Hfr Hrun". *)
+    (* iAssert *)
+    (* (frame_interp rti sr se L (wl ++ wl_save ++ [prelude.W.T_i32] ++ wl_case_i ++ wl2 ++ wlf) fr_saved) *)
+    (*   with "[Hframe]" as "Hframe_saved". *)
+    (* { admit. } (* TODO: Not really sure how to prove this. Definitely need helper lemma *) *)
+    (**)
+    (* edestruct (util.nths_error_exists val_localidxs case_i_val_idxs vs_payload case_i_sum_locals (Forall2_length _ _ _ Hsaved)) as [case_i_vs_payload Hnerr_payload_ci]; try done. *)
+    (**)
+    (* iDestruct (frame_interp_wl_interp with "Hframe_saved") as "%Hwl_saved"; first done. *)
+    (* pose proof (interp_wl_length _ _ _ Hwl_saved) as Hfr_saved_locs_len. *)
+    (**)
+    (* assert (tag_idx < length (f_locs fr_saved)) as Htag_in_fr_saved. *)
+    (* { *)
+    (*   subst tag_idx. *)
+    (*   simpl. *)
+    (*   eapply Nat.lt_le_trans; last done. *)
+    (*   - rewrite app_assoc. *)
+    (*     subst fe. *)
+    (*     instantiate (1 := F). *)
+    (*     repeat rewrite length_app. *)
+    (*     lias. *)
+    (* } *)
+    (**)
+    (* (* Store tag *) *)
+    (* rewrite (app_assoc (map _ _)). *)
+    (* iApply (cwp_seq with "[Hfr Hrun]"). *)
+    (* { *)
+    (*   instantiate (1 := λ fr' vs, ( *)
+    (*     ⌜vs = []⌝ ∗ *)
+    (*     ⌜frame_rel (λ j, j ≠ tag_idx) fr_saved fr'⌝ ∗ *)
+    (*     ⌜f_locs fr' !! tag_idx = Some (VAL_int32 (Wasm_int.Int32.repr tag))⌝ *)
+    (*     )%I). *)
+    (*   iApply (cwp_local_set with "[] [$] [$]"); first done. *)
+    (*   iSplit; first done. *)
+    (*   iSplit. *)
+    (*   - iPureIntro. *)
+    (*     split; last done. *)
+    (*     intros j Hneq. *)
+    (*     simpl. *)
+    (*     rewrite list_lookup_insert_ne; [reflexivity | lia]. *)
+    (*   - iSimpl. *)
+    (*     iPureIntro. *)
+    (*     rewrite list_lookup_insert_eq; try done. *)
+    (* } *)
+    (* iIntros (fr_saved_and_tag w) "(-> & %Hfrel_fr_saved_and_tag & %Hsaved_and_tag) Hfr Hrun". *)
+    (* clear_nils. *)
+    (**)
+    (* (* relate starting frame fr and fr_saved_and_tag *) *)
+    (* pose proof (frame_rel_mask_trans_combine _ _ _ _ _ Hfrel_fr_saved Hfrel_fr_saved_and_tag) as Hfrel_fr_and_fr_saved_and_tag. *)
+    (* simpl in Hfrel_fr_and_fr_saved_and_tag. *)
+    (**)
+    (* assert (frame_rel lmask fr fr_saved_and_tag) as Hfrel_lmask_saved_and_tag. *)
+    (* { *)
+    (*   eapply frame_rel_mask_mono; [| exact Hfrel_fr_and_fr_saved_and_tag]. *)
+    (*   intros i [Hi_lo Hi_hi]. *)
+    (*   split. *)
+    (*   + rewrite Hval_idxs_seq. *)
+    (*     intro Hin. apply elem_of_seq in Hin. lia. *)
+    (*   + unfold tag_idx. rewrite length_app. lia. *)
+    (* } *)
+    (* pose proof Hfrel_fr_and_fr_saved_and_tag as [_ ->]. *)
+    (* iDestruct (labels_interp_mono _ _ _ _ fr_saved_and_tag _ _ _ _ with "Hlabels") as "Hlabels'"; first done. *)
+    (* { *)
+    (*   instantiate (1 := (wlmask (fe_of_context F') (wl ++ wl_save ++ [prelude.W.T_i32]))). *)
+    (*   intros i [Hi_lo Hi_hi]. *)
+    (*   simpl. *)
+    (*   split. *)
+    (*   + exact Hi_lo. *)
+    (*   + rewrite -fe_of_context_labels. *)
+    (*     rewrite !length_app. simpl. *)
+    (*     subst fe. *)
+    (*     lia. *)
+    (* } *)
+    (**)
+    (* assert (Forall2 (λ (i : prelude.W.localidx) (v : value), f_locs fr_saved_and_tag !! localimm i = Some v) *)
+    (*   val_localidxs vs_payload) as Hfr_saved_and_tag_payload. *)
+    (* { *)
+    (*   eapply forall2_lookup_same. *)
+    (*   3: done. *)
+    (*   - intros j Hneq. instantiate (1 := tag_idx) in Hneq. *)
+    (*     destruct Hfrel_fr_saved_and_tag as [-> _]; done. *)
+    (*   - subst val_idxs val_localidxs tag_idx. *)
+    (*     rewrite length_app Nat.add_assoc. *)
+    (*     apply map_seq_forall_localidx_neq. *)
+    (* } *)
+    (**)
+    (* iAssert *)
+    (* (frame_interp rti sr se L (wl ++ wl_save ++ [prelude.W.T_i32] ++ wl_case_i ++ wl2 ++ wlf) fr_saved_and_tag) *)
+    (*   with "[Hframe_saved]" as "Hframe_saved_and_tag". *)
+    (* { admit. } (* TODO: Not really sure how to prove this. Definitely need helper lemma *) *)
+    (**)
+    (* (* Create defaults *) *)
+    (* iApply (cwp_seq with "[Hfr Hrun]"). *)
+    (* { *)
+    (*   eapply cwp_create_defaults in Hcreate_defaults as (_ & _ & _ & Hcreate_defaults). *)
+    (*   iDestruct (Hcreate_defaults with "[$] [$] []") as "Hcreate_defaults". *)
+    (*   { *)
+    (*     by instantiate (1 := λ f vs, (⌜f = fr_saved_and_tag⌝ ∗ ⌜vs = (map default_of_value_type wl_ret)⌝)%I). *)
+    (*   } *)
+    (*   iApply "Hcreate_defaults". *)
+    (* } *)
+    (* iIntros (??) "[-> ->] Hfr Hrun". *)
+    (**)
+    (* (* Case analysis: Is tag 0  *) *)
+    (**)
+    (* apply lookup_lt_Some in Htag_type_lookup as Hi. *)
+    (* destruct tag as [| [|[|]]]; last done. *)
+    (**)
+    (* - (* Case: tag = 0 *) *)
+    (*   (* -------- Case 1 -------- *) *)
+    (*   rewrite (app_assoc (to_consts _)). *)
+    (*   iApply (cwp_seq with "[-]"). *)
+    (*   { *)
+    (*     iApply (compat_case_block_success with "[] [$] [$] [$] [$] [$] [$] [$] [$] [$]"). *)
+    (*     2: instantiate (1 := []). *)
+    (*     all: clear_nils. *)
+    (*     1, 2, 3, 4, 5, 6, 8, 9, 11, 13, 14: done. *)
+    (*     4: iApply "Hsem_es1". *)
+    (*     1: done. *)
+    (*     1: by rewrite length_map. *)
+    (*     by subst val_idxs. *)
+    (*   } *)
+    (*   iIntros (f_es_case_1 vs) "(_ & %Hlen_vs & %Hfrel_new & Hframe & %os & %θ' & Hos & Hvs & Hrt) Hfr Hrun". *)
+    (**)
+    (*   (* -------- Case 2 -------- *) *)
+    (*   rewrite (app_assoc (to_consts _)). *)
+    (*   iApply (cwp_seq with "[Hfr Hrun]"). *)
+    (*   { *)
+    (*     iApply (compat_case_block_fail with "[$] [$]"). *)
+    (*     2, 3, 4, 5, 6, 7, 8, 9, 10: done. *)
+    (*     rewrite -Hsaved_and_tag. *)
+    (*     destruct Hfrel_new as [Hmask _]. *)
+    (*     symmetry. *)
+    (*     apply Hmask. *)
+    (*     subst tag_idx fe. *)
+    (*     unfold wlmask. *)
+    (*     repeat rewrite length_app. *)
+    (*     rewrite -fe_of_context_labels. *)
+    (*     lias. *)
+    (*   } *)
+    (*   iIntros (??) "(-> & ->) Hfr Hrun". *)
+    (**)
+    (*   (* -------- Case 3 -------- *) *)
+    (*   iApply (cwp_wand with "[Hfr Hrun]"). *)
+    (*   { *)
+    (*     iApply (compat_case_block_fail with "[$] [$]"). *)
+    (*     2, 3, 4, 5, 6, 8, 9, 10: done. *)
+    (*     2: done. *)
+    (*     rewrite -Hsaved_and_tag. *)
+    (*     destruct Hfrel_new as [Hmask _]. *)
+    (*     symmetry. *)
+    (*     apply Hmask. *)
+    (*     subst tag_idx fe. *)
+    (*     unfold wlmask. *)
+    (*     repeat rewrite length_app. *)
+    (*     rewrite -fe_of_context_labels. *)
+    (*     lias. *)
+    (*   } *)
+    (*   iIntros (??) "(-> & ->)". *)
+    (*   iFrame. *)
+    (*   iPureIntro. *)
+    (*   rewrite -fe_of_context_labels in Hfrel_new. *)
+    (*   unfold lmask. *)
+    (*   eapply frame_rel_trans. *)
+    (*   + eapply frame_rel_mask_mono; [| exact Hfrel_lmask_saved_and_tag]. *)
+    (*     intros i [Hi_lo Hi_hi]. unfold lmask, wlmask. split; exact Hi_lo || exact Hi_hi. *)
+    (*   + eapply frame_rel_wlmask_mono; [| exact Hfrel_new]. *)
+    (*     rewrite length_app. lia. *)
+    (**)
+    (* - (* Case: tag = 1 *) *)
+    (*   (* -------- Case 1 -------- *) *)
+    (*   rewrite (app_assoc (to_consts _)). *)
+    (*   iApply (cwp_seq with "[Hfr Hrun]"). *)
+    (*   { *)
+    (*     iApply (compat_case_block_fail with "[$] [$]"). *)
+    (*     7: by instantiate (1 := 1). *)
+    (*     2: instantiate (1 := []). *)
+    (*     1, 2, 3, 4, 5, 6, 7, 8: done. *)
+    (*     by rewrite length_map. *)
+    (*   } *)
+    (*   iIntros (??) "(-> & ->) Hfr Hrun". *)
+    (**)
+    (*   iDestruct (labels_interp_mono _ _ _ _ fr_saved_and_tag _ _ _ _ with "Hlabels") as "Hlabels'''"; first done. *)
+    (*   { *)
+    (*     instantiate (1 := (wlmask (fe_of_context F') (wl ++ wl_save ++ [prelude.W.T_i32] ++ wl_case_1))). *)
+    (*     intros i [Hi_lo Hi_hi]. *)
+    (*     simpl. *)
+    (*     split. *)
+    (*     + exact Hi_lo. *)
+    (*     + rewrite -fe_of_context_labels. *)
+    (*       rewrite !length_app. simpl. *)
+    (*       subst fe. *)
+    (*       lia. *)
+    (*   } *)
+    (**)
+    (*   (* -------- Case 2 -------- *) *)
+    (*   rewrite (app_assoc (to_consts _)). *)
+    (*   iApply (cwp_seq with "[-]"). *)
+    (*   { *)
+    (*     iApply (compat_case_block_success with "[] [$] [$] [$] [$] [$] [$] [$] [$] [$]"). *)
+    (*     1, 2, 3, 4, 5, 6, 8, 9, 11, 13, 14: done. *)
+    (*     4: iApply "Hsem_es2". *)
+    (*     1: done. *)
+    (*     1: by rewrite length_map. *)
+    (*     by subst val_idxs. *)
+    (*   } *)
+    (*   iIntros (f_es_case_2 vs) "(_ & %Hlen_vs & %Hfrel_new & Hframe & %os & %θ' & Hos & Hvs & Hrt) Hfr Hrun". *)
+    (**)
+    (*   (* -------- Case 3 -------- *) *)
+    (*   iApply (cwp_wand with "[Hfr Hrun]"). *)
+    (*   { *)
+    (*     iApply (compat_case_block_fail with "[$] [$]"). *)
+    (*     2, 3, 4, 5, 6, 8, 9, 10: done. *)
+    (*     2: done. *)
+    (*     rewrite -Hsaved_and_tag. *)
+    (*     destruct Hfrel_new as [Hmask _]. *)
+    (*     symmetry. *)
+    (*     apply Hmask. *)
+    (*     subst tag_idx fe. *)
+    (*     unfold wlmask. *)
+    (*     repeat rewrite length_app. *)
+    (*     rewrite -fe_of_context_labels. *)
+    (*     lias. *)
+    (*   } *)
+    (*   iIntros (??) "(-> & ->)". *)
+    (*   iFrame. *)
+    (*   iPureIntro. *)
+    (*   rewrite -fe_of_context_labels in Hfrel_new. *)
+    (*   unfold lmask. *)
+    (*   eapply frame_rel_trans. *)
+    (*   + eapply frame_rel_mask_mono; [| exact Hfrel_lmask_saved_and_tag]. *)
+    (*     intros i [Hi_lo Hi_hi]. unfold lmask, wlmask. split; exact Hi_lo || exact Hi_hi. *)
+    (*   + eapply frame_rel_wlmask_mono; [| exact Hfrel_new]. *)
+    (*     rewrite length_app. lia. *)
+    (**)
+    (* - (* Case: tag = 2 *) *)
+    (*   (* -------- Case 1 -------- *) *)
+    (*   rewrite (app_assoc (to_consts _)). *)
+    (*   iApply (cwp_seq with "[Hfr Hrun]"). *)
+    (*   { *)
+    (*     iApply (compat_case_block_fail with "[$] [$]"). *)
+    (*     7: by instantiate (1 := 2). *)
+    (*     2: instantiate (1 := []). *)
+    (*     1, 2, 3, 4, 5, 6, 7, 8: done. *)
+    (*     by rewrite length_map. *)
+    (*   } *)
+    (*   iIntros (??) "(-> & ->) Hfr Hrun". *)
+    (**)
+    (*   (* -------- Case 2 -------- *) *)
+    (*   rewrite (app_assoc (to_consts _)). *)
+    (*   iApply (cwp_seq with "[Hfr Hrun]"). *)
+    (*   { *)
+    (*     iApply (compat_case_block_fail with "[$] [$]"). *)
+    (*     7: by instantiate (1 := 2). *)
+    (*     2: instantiate (1 := wl_case_1). *)
+    (*     1, 2, 3, 4, 5, 6, 7, 8: done. *)
+    (*     by rewrite length_map. *)
+    (*   } *)
+    (*   iIntros (??) "(-> & ->) Hfr Hrun". *)
+    (**)
+    (*   iDestruct (labels_interp_mono _ _ _ _ fr_saved_and_tag _ _ _ _ with "Hlabels") as "Hlabels'''"; first done. *)
+    (*   { *)
+    (*     instantiate (1 := (wlmask (fe_of_context F') (wl ++ wl_save ++ [prelude.W.T_i32] ++ wl_case_1 ++ wl_case_2))). *)
+    (*     intros i [Hi_lo Hi_hi]. *)
+    (*     simpl. *)
+    (*     split. *)
+    (*     + exact Hi_lo. *)
+    (*     + rewrite -fe_of_context_labels. *)
+    (*       rewrite !length_app. simpl. *)
+    (*       subst fe. *)
+    (*       lia. *)
+    (*   } *)
+    (**)
+    (*   (* -------- Case 3 -------- *) *)
+    (*   iApply (cwp_wand with "[-]"). *)
+    (*   { *)
+    (*     iApply (compat_case_block_success with "[] [$] [$] [$] [$] [$] [$] [$] [$] [$]"). *)
+    (*     1, 2, 3, 4, 5, 6, 8, 9, 11, 13, 14: done. *)
+    (*     4: iApply "Hsem_es3". *)
+    (*     1: done. *)
+    (*     1: by rewrite length_map. *)
+    (*     by subst val_idxs. *)
+    (*   } *)
+    (*   iIntros (f_es_case_3 vs) "(_ & %Hlen_vs & %Hfrel_new & Hframe & %os & %θ' & Hos & Hvs & Hrt)". *)
+    (*   iFrame. *)
+    (*   iPureIntro. *)
+    (*   rewrite -fe_of_context_labels in Hfrel_new. *)
+    (*   unfold lmask. *)
+    (*   eapply frame_rel_trans. *)
+    (*   + eapply frame_rel_mask_mono; [| exact Hfrel_lmask_saved_and_tag]. *)
+    (*     intros i [Hi_lo Hi_hi]. unfold lmask, wlmask. split; exact Hi_lo || exact Hi_hi. *)
+    (*   + eapply frame_rel_wlmask_mono; [| exact Hfrel_new]. *)
+    (*     rewrite length_app. lia. *)
   Admitted.
 
 End case.
